theories/Syntax/ListNat.v
@@ -53,6 +53,73 @@ Module ListNat.
 
   Definition map : tm := tFix map_ty map_body.
 
+  (** append : List -> List -> List *)
+  Definition append_ty : tm := tPi list_ty (tPi list_ty list_ty).
+
+  Definition append_body : tm :=
+    (* self : append_ty *)
+    tLam list_ty ( (* l1 *)
+      tLam list_ty ( (* l2 *)
+        tCase 1 (tVar 1) list_ty
+          [ tVar 0; (* nil -> l2 *)
+            (* cons branch: \x:Nat. \xs:List. cons x (append xs l2) *)
+            tLam Examples.nat_ty (
+              tLam list_ty (
+                cons (tVar 1)
+                  (tApp (tApp (tVar 4) (tVar 0)) (tVar 2))
+              ))
+          ]
+      )).
+
+  Definition append : tm := tFix append_ty append_body.
+
+  (** take : Nat -> List -> List *)
+  Definition take_ty : tm := tPi Examples.nat_ty (tPi list_ty list_ty).
+
+  Definition take_body : tm :=
+    (* self : take_ty *)
+    tLam Examples.nat_ty ( (* n *)
+      tLam list_ty ( (* l *)
+        tCase 0 (tVar 1) list_ty
+          [ nil;
+            (* succ branch: \n'. case l of nil -> nil | cons x xs -> cons x (take n' xs) *)
+            tLam Examples.nat_ty (
+              tCase 1 (tVar 1) list_ty
+                [ nil;
+                  tLam Examples.nat_ty (
+                    tLam list_ty (
+                      cons (tVar 1)
+                        (tApp (tApp (tVar 5) (tVar 2)) (tVar 0))
+                    ))
+                ])
+          ]
+      )).
+
+  Definition take : tm := tFix take_ty take_body.
+
+  (** drop : Nat -> List -> List *)
+  Definition drop_ty : tm := tPi Examples.nat_ty (tPi list_ty list_ty).
+
+  Definition drop_body : tm :=
+    (* self : drop_ty *)
+    tLam Examples.nat_ty ( (* n *)
+      tLam list_ty ( (* l *)
+        tCase 0 (tVar 1) list_ty
+          [ tVar 0;
+            (* succ branch: \n'. case l of nil -> nil | cons x xs -> drop n' xs *)
+            tLam Examples.nat_ty (
+              tCase 1 (tVar 1) list_ty
+                [ nil;
+                  tLam Examples.nat_ty (
+                    tLam list_ty (
+                      tApp (tApp (tVar 5) (tVar 2)) (tVar 0)
+                    ))
+                ])
+          ]
+      )).
+
+  Definition drop : tm := tFix drop_ty drop_body.
+
   (** length : List -> Nat *)
   Definition length_ty : tm := tPi list_ty Examples.nat_ty.
 
